share/steel/examples/pulse/parallel/Async.fsti
@@ -1,0 +1,30 @@
+module Async
+
+open Pulse.Lib.Pervasives
+
+val asynch (a:Type0) (post : a -> vprop) : Type0
+
+val async_joinable
+  (#a : Type0)
+  (#post : a -> vprop)
+  (h : asynch a post)
+  : vprop
+
+```pulse
+val
+fn async
+  (#a : Type0) (#pre : vprop) (#post : (a -> vprop))
+  (f : (unit -> stt a pre post))
+requires pre
+returns h : asynch a post
+ensures async_joinable h
+```
+
+```pulse
+val
+fn await (#a : Type0) (#post : (a -> vprop))
+  (h : asynch a post)
+requires async_joinable h
+returns x : a
+ensures post x
+```
