share/steel/examples/pulse/parallel/ParallelFor.fsti
@@ -1,0 +1,62 @@
+module ParallelFor
+
+open Pulse.Lib.Pervasives
+
+let rec range (p : nat -> vprop) (i j : nat) : Tot vprop (decreases j-i) =
+  if i < j
+  then p i ** range p (i+1) j
+  else emp
+
+```pulse
+val
+fn
+parallel_for
+  (pre : (nat -> vprop))
+  (post : (nat -> vprop))
+  (f : (i:nat -> stt unit (pre i) (fun () -> (post i))))
+  (n : pos)
+  requires range pre 0 n
+  ensures range post 0 n
+```
+
+(* Alternative; not splitting the pool_alive resource. We are anyway
+spawning sequentially. *)
+```pulse
+val
+fn
+parallel_for_alt
+  (pre : (nat -> vprop))
+  (post : (nat -> vprop))
+  (f : (i:nat -> stt unit (pre i) (fun () -> (post i))))
+  (n : pos)
+  requires range pre 0 n
+  ensures range post 0 n
+```
+
+```pulse
+val
+fn
+parallel_for_wsr
+  (pre : (nat -> vprop))
+  (post : (nat -> vprop))
+  (full_pre : (nat -> vprop))
+  (full_post : (nat -> vprop))
+  (f : (i:nat -> stt unit (pre i) (fun () -> post i)))
+  (unfold_pre : (i:nat -> stt_ghost unit emp_inames (full_pre (i+1)) (fun () -> pre i ** full_pre i)))
+  (fold_post : (i:nat -> stt_ghost unit emp_inames (post i ** full_post i) (fun () -> full_post (i+1))))
+  (n : pos)
+  requires full_pre n ** full_post 0
+  ensures full_pre 0 ** full_post n
+```
+
+```pulse
+val
+fn
+parallel_for_hier
+  (pre : (nat -> vprop))
+  (post : (nat -> vprop))
+  (f : (i:nat -> stt unit (pre i) (fun () -> (post i))))
+  (n : pos)
+  requires range pre 0 n
+  ensures range post 0 n
+```
